theories/elpi_test.v
@@ -40,7 +40,7 @@ Definition tester l r :=
 Goal forall B B0,
 let f x := (TA (call x)) in
 let g x := ([:: (call x) ]%SEQ) in
-  tester (And (Or OK empty (f B)) (g B0) KO) 
+  tester (And (Or (Some OK) empty (f B)) (g B0) KO) 
     ((empty, (call B,[::]) ::: ((call B0,[::]) ::: nilC)) ::: nilC).
 Proof.
   by move=> //.
@@ -53,7 +53,7 @@ Goal forall A B D0 D,
   let f x := (TA (call x)) in
   let g x := ([::call x]%SEQ) in
   tester 
-    (And (Or ((Or (TA cut) empty (f A))) empty (f B)) (g D0) (f D)) 
+    (And (Or ((Some (Or (Some (TA cut)) empty (f A)))) empty (f B)) (g D0) (f D)) 
     (of_alt [:: 
       [:: (cut, of_alt [:: [:: (callN B); (callN D0)]%SEQ]); (callN D)];
       [:: (callN A); (callN D0)]; 
@@ -69,7 +69,7 @@ Goal forall B C D E F,
   let g x := ([::call x]%SEQ) in
   (* (A \/_{empty} B) /\_C ((! \/_{empty} D) /\_{E} F) *)
   tester 
-    (And (Or OK empty (f B)) (g C) (And (Or (TA cut) empty (f D)) (g E) (f F)))
+    (And (Or (Some OK) empty (f B)) (g C) (And (Or (Some (TA cut)) empty (f D)) (g E) (f F)))
     (of_alt [:: 
       [:: (cut, (of_alt [:: [:: callN B; callN C]])); callN F];
       [:: callN D; callN E]; 
@@ -99,7 +99,7 @@ Goal forall A B C0 C,
   let g x := ([::call x]%SEQ) in
   (* (((! \/ A) \/ B)) /\ (! \/ C)*)
   tester 
-    (And (Or ((Or (TA cut) empty (f A))) empty (f B)) (g C0) (Or (TA cut) empty (f C)))
+    (And (Or ((Some (Or (Some (TA cut)) empty (f A)))) empty (f B)) (g C0) (Or (Some (TA cut)) empty (f C)))
     (of_alt[:: 
       [::(cut, (of_alt [:: [:: callN B; callN C0]])); (cut, (of_alt [::[:: callN A; callN C0]; [:: callN B; callN C0]]))];
       [::(cut, (of_alt [:: [:: callN B; callN C0]])); callN C];
@@ -115,7 +115,7 @@ Goal forall A B0,
     (* (OK \/ A) /\_B0 OK *)
   let f x := (TA (call x)) in
   let g x := ([::call x]%SEQ) in
-  tester (And (Or OK empty (f A)) (g B0) OK) (of_alt [::[::]; [::callN A; callN B0]]%SEQ).
+  tester (And (Or (Some OK) empty (f A)) (g B0) OK) (of_alt [::[::]; [::callN A; callN B0]]%SEQ).
 Proof.
   move=> A B0 p.
   rewrite/t2l//=.
@@ -125,7 +125,7 @@ Goal forall A B0,
   (* (KO \/ B) /\_b0 B0  *)
   let f x := (TA (call x)) in
   let g x := ([::call x]%SEQ) in
-  tester (And (Or KO empty (f A)) (g B0) (f B0))
+  tester (And (Or (Some KO) empty (f A)) (g B0) (f B0))
   (of_alt [::[::callN A; callN B0]]%SEQ).
 Proof.
   move=> A B0 p.
@@ -137,8 +137,8 @@ Goal forall x y z w a,
   let g x := ([::call x]%SEQ) in
   tester (
     And 
-      (Or (f x) empty (f y)) (g a) 
-      (Or (f z) empty (f w))) 
+      (Or (Some (f x)) empty (f y)) (g a) 
+      (Or (Some (f z)) empty (f w))) 
     (of_alt [:: [:: callN x; callN z];
     [:: callN x; callN w];
     [:: callN y; callN a]]%SEQ).
@@ -151,8 +151,8 @@ Goal forall z w a,
   let f x := (TA (call x)) in
   tester (
     And 
-      (Or OK empty KO) (g a) 
-      (Or (f z) empty (f w))) 
+      (Or (Some OK) empty KO) (g a) 
+      (Or (Some (f z)) empty (f w))) 
     (of_alt [:: [:: callN z]; [:: callN w]]%SEQ).
 Proof.
   move=>p z w a.
@@ -165,8 +165,8 @@ Goal forall a b c d,
   let f x := (TA (call x)) in
   tester (
     And 
-      (Or KO empty (f a)) (g b) 
-      (Or (f c) empty (f d))) 
+      (Or (Some KO) empty (f a)) (g b) 
+      (Or (Some (f c)) empty (f d))) 
     (* [:: [:: callN a; call b] ]. *)
     (of_alt [:: [:: callN a; callN c]; [::callN a; callN d] ]%SEQ).
 Proof.
@@ -178,7 +178,7 @@ Goal forall a b,
 (* (! \/ a) \/ b *)
   tester (
     Or 
-      (Or (TA cut) empty (TA (call a))) empty
+      (Some (Or (Some (TA cut)) empty (TA (call a)))) empty
       (TA (call b)))
   (of_alt [:: [:: (cut, (of_alt[:: [:: callN b]]))]; [:: callN a]; [:: callN b]]%SEQ).
 Proof.
@@ -207,7 +207,7 @@ Qed. *)
 
 Goal forall A1 A2 B0 C0 B,
   let f x := (TA (call x)) in
-  tester (And (Or (f A1) empty (f A2)) (g B0) (And KO (g C0) (f B)))
+  tester (And (Or (Some (f A1)) empty (f A2)) (g B0) (And KO (g C0) (f B)))
   (of_alt [:: [:: callN A2 ; callN B0 ]]%SEQ).
 Proof.
   move=> * /=.
@@ -217,7 +217,7 @@ Qed.
 Goal forall b0 a b c, 
   tester (
     Or 
-      (Or (And (TA (call c)) (g b0) (TA cut)) empty (TA (call a))) empty
+      (Some (Or (Some (And (TA (call c)) (g b0) (TA cut))) empty (TA (call a)))) empty
       (TA (call b)))
   (of_alt[:: [:: callN c; (cut, (of_alt[:: [:: callN b]]))]; [:: callN a]; [:: callN b]]%SEQ).
 Proof.
@@ -229,7 +229,7 @@ Qed.
 Goal forall B C Res,
   let f x := (TA (call x)) in
   (* (OK \/ B) /\ (! \/ C) -> [cut_[B,Reset]; C; (B, Reset)] *)
-  tester (And (Or OK empty (f B)) (g Res) (Or (TA cut) empty (f C))) 
+  tester (And (Or (Some OK) empty (f B)) (g Res) (Or (Some (TA cut)) empty (f C))) 
     (of_alt[::[::(cut, (of_alt[::[:: callN B; callN Res]]))]; [::callN C]; [:: callN B; callN Res]]%SEQ).
 Proof.
   move=> B C Res p.
@@ -240,7 +240,7 @@ Qed.
 Goal forall B C Res Reempty,
   let f x := (TA (call x)) in
   (* (OK \/ B) /\ (! /\ C) -> [cut_[]; C; (B, Reset)] *)
-  tester (And (Or OK empty (f B)) (g Res) (And (TA cut) (g Reempty) (f C))) 
+  tester (And (Or (Some OK) empty (f B)) (g Res) (And (TA cut) (g Reempty) (f C))) 
     (of_alt[::[::(cut, nilC); callN C]; [:: callN B; callN Res]]%SEQ).
 Proof.
   move=> B C Res Reempty p/=.
@@ -251,7 +251,7 @@ Qed.
 Goal forall A B C C0,
   let f x := (TA (call x)) in
   (* (A /\ ((! \/ B) \/ C) *)
-  tester (And (f A) (g C0) (Or (Or (TA cut) empty (f B)) empty (f C))) 
+  tester (And (f A) (g C0) (Or (Some (Or (Some (TA cut)) empty (f B))) empty (f C))) 
   (of_alt [:: 
     [:: callN A; (cut, (of_alt[:: [:: callN C]]))]; 
     [:: callN A; callN B]; 
@@ -266,7 +266,7 @@ Goal forall A B C D E,
   let f x := (TA (call x)) in
   (* (A \/_{empty} B) /\_C ((! \/_{empty} D) \/_{empty} E) *)
   tester 
-    (And (Or (f A) empty (f B)) (g C) (Or (Or (TA cut) empty (f D)) empty (f E))) 
+    (And (Or (Some (f A)) empty (f B)) (g C) (Or (Some (Or (Some (TA cut)) empty (f D))) empty (f E))) 
     (of_alt[:: 
     [:: callN A; (cut, (of_alt [:: [:: callN E]; [:: callN B; callN C]]))];
     [:: callN A; callN D]; [:: callN A; callN E];
@@ -287,7 +287,7 @@ Goal forall B C D E,
   let f x := (TA (call x)) in
   (* (OK \/_{empty} B) /\_C ((! \/_{empty} D) /\_{E} !) *)
   tester 
-    (And (Or OK empty (f B)) (g C) (And (Or (TA cut) empty (f D)) (g E) (TA cut))) 
+    (And (Or (Some OK) empty (f B)) (g C) (And (Or (Some (TA cut)) empty (f D)) (g E) (TA cut))) 
     (of_alt [:: 
       [:: (cut, (of_alt[:: [:: callN B; callN C]])); (cut, nilC) ];
       [:: callN D; callN E]; 
@@ -302,7 +302,7 @@ Goal forall A B C,
   let f x := (TA (call x)) in
   (* ((! \/ ! \/ A) \/ B) \/ C *)
   tester
-    (Or (Or (Or (TA cut) empty ((Or (TA cut) empty (f A)))) empty (f B)) empty (f C))
+    (Or (Some (Or (Some (Or (Some (TA cut)) empty ((Or (Some (TA cut)) empty (f A))))) empty (f B))) empty (f C))
     (of_alt[:: 
       [::(cut, (of_alt[:: [:: callN B]; [::callN C]]))];
       [::(cut, (of_alt[:: [:: callN B]; [::callN C]]))];
@@ -319,7 +319,7 @@ Goal forall A B C,
   let f x := (TA (call x)) in
   (* ((! \/ ! \/ A) \/ B) \/ C *)
   tester 
-    (Or (Or (Or (And (TA cut) ([::]) OK) empty ((Or (TA cut) empty (f A)))) empty (f B)) empty (f C)) 
+    (Or (Some (Or (Some (Or (Some (And (TA cut) ([::]) OK)) empty ((Or (Some (TA cut)) empty (f A))))) empty (f B))) empty (f C)) 
     (of_alt[:: 
       [::(cut, (of_alt[:: [:: callN B]; [::callN C]]))];
       [::(cut, (of_alt[:: [:: callN B]; [::callN C]]))];
@@ -337,7 +337,7 @@ Goal forall A B C D0 D,
   let f x := (TA (call x)) in
   (* (((! \/ ! \/ A) \/ B) \/ C) /\ D*)
   tester
-    (And (Or (Or (Or (TA cut) empty ((Or (TA cut) empty (f A)))) empty (f B)) empty (f C)) (g D0) (f D))
+    (And (Or (Some (Or (Some (Or (Some (TA cut)) empty ((Or (Some (TA cut)) empty (f A))))) empty (f B))) empty (f C)) (g D0) (f D))
     (of_alt[:: 
       [::(cut, (of_alt [:: [:: callN B; callN D0]; [::callN C; callN D0]])); callN D];
       [::(cut, (of_alt [:: [:: callN B; callN D0]; [::callN C; callN D0]])); callN D0];
@@ -354,7 +354,7 @@ Goal forall X A B C D0 D,
   let f x := (TA (call x)) in
   (* ((X \/ ((! \/ ! \/ A) \/ B) \/ C)) /\ D*)
   tester 
-    (And (Or (f X) empty (Or (Or (Or (TA cut) empty ((Or (TA cut) empty (f A)))) empty (f B)) empty (f C))) (g D0) (f D))
+    (And (Or (Some (f X)) empty (Or (Some (Or (Some (Or (Some (TA cut)) empty ((Or (Some (TA cut)) empty (f A))))) empty (f B))) empty (f C))) (g D0) (f D))
     (of_alt[:: 
       [:: callN X; callN D];
       [::(cut, (of_alt[:: [:: callN B; callN D0]; [::callN C; callN D0]])); callN D0];
@@ -372,7 +372,7 @@ Goal forall B0 A B C D,
   let f x := (TA (call x)) in
   (* (((A /\ (! \/ B)) \/ C \/ D)) *)
   tester 
-    (Or (Or (f C) empty (And (f A) (g B0) (Or (TA cut) empty (f B)))) empty (f D))
+    (Or (Some (Or (Some (f C)) empty (And (f A) (g B0) (Or (Some (TA cut)) empty (f B))))) empty (f D))
     (of_alt[:: 
       [:: callN C]; 
       [:: callN A; (cut, (of_alt[:: [:: callN D]]))]; 
@@ -387,7 +387,7 @@ Goal forall A B C,
   let f x := (TA (call x)) in
   (* (((! \/ A) \/ !) \/ B) \/ C *)
   tester 
-    (Or (Or (Or (Or (TA cut) empty (f A)) empty (TA cut)) empty (f B)) empty (f C))
+    (Or (Some (Or (Some (Or (Some (Or (Some (TA cut)) empty (f A))) empty (TA cut))) empty (f B))) empty (f C))
     (of_alt[:: 
       [::(cut, (of_alt[::[::(cut, (of_alt[::[::callN B]; [::callN C]]))]; [::callN B]; [::callN C]]))];
       [::callN A];
@@ -401,7 +401,7 @@ Proof.
   rewrite//.
 Qed.
 Goal forall p l,
-  let s := ((Or (Or Dead empty (TA cut)) empty OK)) in
+  let s := ((Or (Some (Or None empty (TA cut))) empty OK)) in
   let bt := of_alt([::]%SEQ :: l) in
   t2l s empty (of_alt l) = of_alt[:: [:: (cut, bt)]; [::]]%SEQ /\ 
     t2l (odflt KO (next_alt true (step u p fset0 empty s).2)) empty (of_alt l) ++ (of_alt l) = bt.
